% Equation 1
\begin{dmath}
{{c}}_{t}^{\left(-{{\sigma}}\right)}=\frac{{{\beta}}}{{{\gamma_x}}}\, {{c}}_{t+1}^{\left(-{{\sigma}}\right)}\, \left({{\alpha}}\, \exp\left({{z}}_{t+1}\right)\, \left(\frac{{{k}}_{t}}{{{l}}_{t+1}}\right)^{{{\alpha}}-1}+1-{{\delta}}\right)
\end{dmath}
% Equation 2
\begin{dmath}
\frac{{{\psi}}\, {{c}}_{t}^{{{\sigma}}}}{1-{{l}}_{t}}={{w}}_{t}
\end{dmath}
% Equation 3
\begin{dmath}
{{\gamma_x}}\, {{k}}_{t}=\left(1-{{\delta}}\right)\, {{k}}_{t-1}+{{i}}_{t}
\end{dmath}
% Equation 4
\begin{dmath}
{{y}}_{t}={{c}}_{t}+{{i}}_{t}+{{\bar G}}\, \exp\left({{\hat g}}_{t}\right)
\end{dmath}
% Equation 5
\begin{dmath}
{{y}}_{t}=\exp\left({{z}}_{t}\right)\, {{k}}_{t-1}^{{{\alpha}}}\, {{l}}_{t}^{1-{{\alpha}}}
\end{dmath}
% Equation 6
\begin{dmath}
{{w}}_{t}=\frac{{{y}}_{t}\, \left(1-{{\alpha}}\right)}{{{l}}_{t}}
\end{dmath}
% Equation 7
\begin{dmath}
{{r}}_{t}=\frac{{{y}}_{t}\, {{\alpha}}\, 4}{{{k}}_{t-1}}
\end{dmath}
% Equation 8
\begin{dmath}
{{z}}_{t}={{\rho_z}}\, {{z}}_{t-1}+{{\varepsilon_z}}_{t}
\end{dmath}
% Equation 9
\begin{dmath}
{{\hat g}}_{t}={{\rho_g}}\, {{\hat g}}_{t-1}+{{\varepsilon_g}}_{t}
\end{dmath}
% Equation 10
\begin{dmath}
{{\log(y)}}_{t}=\log\left({{y}}_{t}\right)
\end{dmath}
% Equation 11
\begin{dmath}
{{\log(k)}}_{t}=\log\left({{k}}_{t}\right)
\end{dmath}
% Equation 12
\begin{dmath}
{{\log(c)}}_{t}=\log\left({{c}}_{t}\right)
\end{dmath}
% Equation 13
\begin{dmath}
{{\log(l)}}_{t}=\log\left({{l}}_{t}\right)
\end{dmath}
% Equation 14
\begin{dmath}
{{\log(w)}}_{t}=\log\left({{w}}_{t}\right)
\end{dmath}
% Equation 15
\begin{dmath}
{{\log(i)}}_{t}=\log\left({{i}}_{t}\right)
\end{dmath}
